\chapter{Constant electromagnetic fields}\label{c5}
\begin{enumerate}
\item If the fields are independent of time then they obey
\begin{eqnarray}
\dive\vec{E} &=& 4\pi\rho \label{c5e1} \\
\curl\vec{E} &=& 0 \label{c5e2} \\
\dive\vec{H} &=& 0 \label{c5e3} \\
\curl\vec{H} &=& 4\pi\frac{\vec{J}}{c}. \label{c5e4}
\end{eqnarray}
The symmetry of the situation reveals itself if we note the correspondence $\vec{E}
\mapsto \vec{H}$ and $\rho \mapsto \vec{J}/c$ and $\dive \mapsto \curl$. Equations
\eqref{c5e2} and \eqref{c5e3} suggest that
\begin{eqnarray}
\vec{E} &=& -\grad\phi \label{c5e5} \\
\vec{H} &=& \curl\vec{A} \label{c5e6}
\end{eqnarray}
which is understandable if we note that only the time component of $J^\mu$ 
determines $\vec{E}$ and its space component determines $\vec{H}$. Therefore,
only the time component of $\vec{A}^\mu$ suffices to describe the electric
field and its space component suffices to describe the magnetic field.

\item From equations \eqref{c5e1} and \eqref{c5e5} we have
\begin{equation}\label{c5e7}
\nabla^2\phi = -4\pi\rho.
\end{equation}
In region where there are no charges, the potential satisfies Laplace's equation
\begin{equation}\label{c5e8}
\nabla^2\phi = 0.
\end{equation}
This equation immediately implies that the potential function cannot have a local
minimum or a maximum. The nature of extremum of a function of three variables is
determined by its Hessian matrix. It is a minimum (maximum) if the Hessian matrix
is positive (negative) definite. Since the trace of a matrix is the sum of its
eigenvalues, we have an equivalent condition that the trace of the Hessian matrix
is positive (negative) for an extremum to be a minimum (maximum). But the trace
of Hessian is $\nabla^2\phi$ evaluated at the extremum. If $\phi$ is a solution
of Laplace's equation \eqref{c5e8}, then the Hessian can never be positive or
negative definite.

\item The field of a point charge can be derived using Gauss' law. Let the point
charge be at $\vec{r}^\op$. In order to find the field at $\vec{r}$, we consider
a sphere centred at $\vec{r}^\op$ and passing through $\vec{r}$. As the space is
isotropic, we expect the magnitude of $\vec{E}$ to be the same at all points on the
sphere and its direction along $\vec{r} - \vec{r}^\op$. Therefore,
\[
4\pi |\vec{r} - \vec{r}^\op|^2 = q
\]
or
\begin{equation}\label{c5e9}
\vec{E} = \frac{q}{|\vec{r} - \vec{r}^\op|^3}(\vec{r} - \vec{r}^\op).
\end{equation}
If we define
\begin{equation}\label{c5e10}
\vec{R} = \vec{r} - \vec{r}^\op
\end{equation}
then we can write \eqref{c5e9} simply as
\begin{equation}\label{c5e11}
\vec{E} = \frac{q}{R^3}\vec{R} = \frac{q}{R^2}\uv{R}.
\end{equation}
Equation \eqref{c5e11} is \emph{Coulomb's law}. The potential of this field is
\begin{equation}\label{c5e12}
\phi = \frac{q}{R}.
\end{equation}
If there are discrete, point charges at $\vec{r}_a$ then the field due to all of 
them is
\begin{equation}\label{c5e13}
\vec{E} = \sum_a \frac{q_a}{R_a^2}\uv{R_a},
\end{equation}
where $\vec{R}_a = \vec{r}^\op - \vec{r}$. The potential is
\begin{equation}\label{c5e14}
\phi = \sum_a\frac{q_a}{R_a}.
\end{equation}
For a continuum of charges, \eqref{c5e11} and \eqref{c5e12} generalise to
\begin{eqnarray}
\phi(\vec{r}) &=& \int\frac{\rho(\vec{r}^\op)}{R}dV \label{c5e15} \\
\vec{E}(\vec{r}) &=& \int\frac{\rho(\vec{r}^\op)}{R^2}\uv{R}dV  \label{c5e16}
\end{eqnarray}

\item For a point charge, $\rho = q\delta(\vec{R})$. In this case, \eqref{c5e7}
becomes,
\[
\nabla^2\phi = 4\pi q\delta(\vec{R}).
\]
From \eqref{c5e12}, we also have
\begin{equation}\label{c5e17}
\nabla^2\left(\frac{1}{R}\right) = -4\pi\delta(\vec{R}).
\end{equation}

\item In the absence of magnetic field, the energy density is
\begin{equation}\label{c5e18}
W = \frac{1}{8\pi}\int E^2dV.
\end{equation}
From \eqref{c5e5},
\[
W = -\frac{1}{8\pi}\int\vec{E}\cdot\grad\phi dV.
\]
Since $\dive(\phi\vec{E}) = \grad\phi\cdot\vec{E} + \phi\dive\vec{E}$, we have
\begin{eqnarray*}
W &=& \frac{1}{8\pi}\int\phi\dive\vec{E}dV - \frac{1}{8\pi}\int\dive(\phi\vec{E})dV \\
  &=& \frac{1}{8\pi}\int\phi\dive\vec{E}dV - \frac{1}{8\pi}\oint \phi\vec{E}\cdot d\vec{f}.
\end{eqnarray*}
The potential goes as $O(r^{-1})$ and the field as $O(r^{-2})$ so that the surface
integral goes as $O(r^{-1})$. If we choose a large enough surface the second 
integral can be made as small as we desire. Thus, we have
\[
W = \frac{1}{8\pi}\int\phi\dive\vec{E}dV
\]
or using \eqref{c5e1},
\begin{equation}\label{c5e19}
W = \frac{1}{2}\int\rho\phi dV.
\end{equation}
If the charge density consists od point charges, equation \eqref{c5e19} becomes
\begin{equation}\label{c5e20}
W = \sum_a q_a\phi(\vec{r}_a),
\end{equation}
where $\phi(\vec{r}_a)$ is the potential due to all charges at the point 
$\vec{r}_a$ where the charge $q_a$ is located. This formula immediately runs 
into a tricky situation.

\item The potential $\phi$ due to a charge $q$ at $\vec{r}^\op$ at the same point
is infinity according to \eqref{c5e12}. As a result, from \eqref{c5e20}, a point
charge has infinite energy and therefore an infinite mass. To avoid such an absurd
result, we say that the laws of classical electrodynamics are not applicable at
extremely short distances. In fact, we cannot even ask the question if the mass of
a charge has electrodynamic origin, that is, it exists because of electrodynamic
energy.

The energy of a uniformly charged sphere of radius $s$ can be computed as follow.
We first note that its charge density is
\begin{equation}\label{c5e21}
\rho = \frac{Q}{\frac{4\pi}{3}s^3}.
\end{equation}
The field due to a sphere of radius $r$ and a uniform charge density $\rho$ at 
points on and outside it is as if the entire charge was concentrated at its 
centre. If $q(r)$ is the charge in a sphere of radius $r$ then the energy
of a charge $dq$ at a distance $r$ from it is
\[
dU = \frac{qdq}{r},
\]
where 
\[
q = \frac{4\pi}{3}r^3 \rho
\]
and $dq = 4\pi r^2 dr$. Thus,
\[
dU = \frac{16\pi^2}{3}\rho^2 r^4dr
\]
and the energy of the entire sphere is
\begin{equation}\label{c5e22}
U = \int_0^s dU = \frac{3}{5}\frac{Q^2}{s}.
\end{equation}
If we consider an elementary charge $q$ to have an infinitesimal radius $r_0$ and
mass $m$ then if the mass has electrodynamic origin,
\[
mc^2 = \frac{3}{5}\frac{q^2}{s}.
\]
Ignoring the factor of $3/5$, the ``classical radius'' of the charge $q$ is defined
to be
\begin{equation}\label{c5e23}
s = \frac{q}{m} c^2.
\end{equation}

\item Quantum effects become important at distance of the order of $\hslash/mc$. The
ratio of this distance to the classical radius of an electron is
\[
\frac{\hslash}{mc}\frac{mc^2}{e^2} = \frac{\hslash c}{e^2} = \frac{1}{\alpha}
\approx 137,
\]
where $\alpha$ is the fine-structure constant. Thus, quantum effects must be taken
into account at distances much larger than the ``classical radius'' of the electron. 
The lower limit of the applicability of classical electrodynamics is much larger 
than the classical electron radius.

\item To avoid the tricky questions of self-energy of elementary charges, we write
the potential $\phi(\vec{r}_a)$ in equation \eqref{c5e20} as
\begin{equation}\label{c5e24}
\phi(\vec{r}_a) = \sum_{b \ne a} \frac{q_b}{R_{ab}},
\end{equation}
where $R_{ab} = |\vec{r}_a - \vec{r}_b|$.

\item We next consider the field of a charge $q$ moving with a uniform velocity
$\vec{v}$. We align the axes such that $\vec{v} = v\uv{x}$ and call the frame
moving with the charge $K^\op$. Let $K$ be the laboratory frame in with axes 
parallel to those of $K^\op$ and let their origins coincide at $t = 0$. Let $P$
be a field point with coordinates $(x^\op, y^\op, z^\op)$ in $K^\op$. Then the
scalar potential at $P$ in $K^\op$ is
\begin{equation}\label{c5e25}
\phi^\op = \frac{q}{R^\op},
\end{equation}
where 
\begin{equation}\label{c5e26}
R^\op = \sqrt{{x^\op}^2 + {y^\op}^2 + {z^\op}^2}
\end{equation}
and the vector potential is
\begin{equation}\label{c5e27}
\vec{A}^\op = 0.
\end{equation}
Thus,
\begin{equation}\label{c5e28}
{A^\op}^\mu = \left(\frac{q}{R^\op}, 0, 0, 0\right).
\end{equation}
From \eqref{c1e46}, the 4-potential in $K$ is
\begin{equation}\label{c5e29}
A^\mu = \left(\gamma\frac{q}{R^\op}, \beta\gamma\frac{q}{R^\op}, 0, 0\right),
\end{equation}
where
\begin{eqnarray*}
\vec{\beta} &=& \frac{\vec{v}}{c} \\
\gamma &=& \frac{1}{\sqrt{1 - \beta^2}}.
\end{eqnarray*}
However, \eqref{c5e29} is not a correct expression because we continue to have
$R^\op$ in it. The relation between $(x, y, z)$ and $(x^\op, y^\op, z^\op)$ is
given the Lorentz transformation
\[
x^\op = \gamma(x - vt) \;;\; y^\op = y \;;\; z^\op = z
\]
so that
\begin{equation}\label{c5e30}
{R^\op}^2 = \gamma^2(x - vt)^2 + (y^2 + z^2).
\end{equation}
We define a function $R^\ast$ of the coordinates $x, y, z$ as
\begin{equation}\label{c5e31}
R^\ast(x, y, z) = \sqrt{(x - vt)^2 + (1 - \beta^2)(y^2 + z^2)}
\end{equation}
so that
\begin{equation}\label{c5e32}
\frac{R^\op(x^\op, y^\op, z^\op)}{\gamma} = R^\ast(x, y, z)
\end{equation}
and the partial Lorentz transformation of \eqref{c5e29} can be completed to
\begin{equation}\label{c5e33}
A^\mu = \left(\frac{q}{R^\ast}, \beta\frac{q}{R^\ast}, 0, 0\right)
\end{equation}
or
\begin{eqnarray}
\phi(x, y, z) &=& \frac{q}{R^\ast} \label{c5e34} \\
\vec{A}(x, y, z) &=& \frac{q\vec{v}}{cR^\ast} \label{c5e35}
\end{eqnarray}

\item The electric and magnetic fields in $K^\op$ frame are
\begin{eqnarray}
\vec{E}^\op &=& \frac{q}{{R^\op}^3}\vec{R}^\op \label{c5e36} \\
\vec{H}^\op &=& 0 \label{c5e37}
\end{eqnarray}
We use equations \eqref{c3e81} to \eqref{c3e83} to get the electric field in the
$K$ frame.
\begin{eqnarray}
E_x &=& E_x^\op \label{c5e38} \\
E_y &=& \gamma E_y^\op \label{c5e39} \\
E_z &=& \gamma E_z^\op \label{c5e40}
\end{eqnarray}
Using \eqref{c5e36} we get
\begin{eqnarray}
E_x &=& \frac{q}{{R^\op}^3}x^\op \label{c5e41} \\
E_y &=& \gamma\frac{q}{{R^\op}^3}y^\op \label{c5e42} \\
E_z &=& \gamma\frac{q}{{R^\op}^3}z^\op \label{c5e43}
\end{eqnarray}
These equations are not satisfactory because their rhs are written in terms of
the primed coordinates. Using $R^\op = \gamma R^\ast$ from \eqref{c5e32} and the
Lorentz transformation formulae
\begin{eqnarray}
E_x &=& \frac{q}{{R^\ast}^3}\frac{x - vt}{\gamma^2} \label{c5e44} \\
E_y &=& \frac{q}{{R^\ast}^3}\frac{y}{\gamma^2} \label{c5e45} \\
E_z &=& \frac{q}{{R^\ast}^3}\frac{z}{\gamma^2} \label{c5e46}
\end{eqnarray}
so that
\begin{equation}\label{c5e47}
\vec{E} = (1 - \beta^2)\frac{q}{{R^\ast}^3}\vec{R},
\end{equation}
where
\begin{equation}\label{c5e48}
\vec{R} = (x - vt)\uv{x} + y\uv{y} + z\uv{z}.
\end{equation}
If $\theta$ is the angle between $\vec{R}$ and $\vec{v}$ then
\begin{equation}\label{c5e49}
\vec{v}\cdot\vec{R} = v(x - vt) = vR\cos\theta \Rightarrow x - vt = R\cos\theta
\end{equation}
so that,
\begin{equation}\label{c5e50}
y^2 + z^2 = R^2 - (x - vt)^2 = R^2\sin^2\theta.
\end{equation}
From \eqref{c5e31}, \eqref{c5e49} and \eqref{c5e50} we get
\begin{equation}\label{c5e51}
{R^\ast}^2 = R^2\cos^2\theta + (1 - \beta^2)R^2\sin^2\theta = 
R^2(1 - \beta^2\sin^2\theta).
\end{equation}
We can now write \eqref{c5e47} solely in terms of $\vec{R}$ as
\begin{equation}\label{c5e52}
\vec{E} = \frac{q\vec{R}}{R^3} \frac{1 - \beta^2}{(1 - \beta^2\sin^2\theta)^{3/2}}.
\end{equation}
Note that $\vec{R}$ is the position of the (moving) charge in $K$ frame.

\item Lorentz transformation of $\vec{E}$ and $\vec{H}$ are a consequence of the
transformation properties of the field tensor. One should use \eqref{c3e81} to
\eqref{c3e84} instead of evaluating $-\grad\phi$ with $\phi$ given by \eqref{c5e34}.
That is, although
\[
\phi^\op = \frac{q}{R^\op} \mapsto \phi = \frac{q}{R^\ast},
\]
the mapping
\[
-\grad^\op\phi^\op \mapsto -\grad\phi
\]
does not hold.

\item In \eqref{c5e52}, $\theta$ is the angle between the radius vector of the
field point $\vec{R}$ and the direction of motion. The magnitude of the field
is
\begin{equation}\label{c5e53}
E = \frac{q}{R^2}\frac{1 - \beta^2}{(1 - \beta^2\sin^2\theta)^{3/2}}
\end{equation}
Figure \ref{c5f1} shows how the magnitude of the electric field varies with 
$\theta$ for different values of $\beta$. As the speed of the charge approaches
$c$, the electric field gets increasingly concentrated along the directions
perpendicular to the motion of the particle.
\begin{figure}[!ht]
\includegraphics[scale=0.8]{ex2}
\caption{$E(\theta)$}
\label{c5f1}
\end{figure}
For an observer in the $K$ frame, the charge in motion creates an electric current
and therefore expects to observe magnetic field. In fact, equations \eqref{c3e84}
to \eqref{c3e86} give
\begin{eqnarray}
H_x &=& 0 \label{c5e54} \\
H_y &=& -\gamma\beta E^\op_z \label{c5e55} \\
H_z &=& \gamma\beta E^\op_y \label{c5e56}
\end{eqnarray}
Since $\beta = v/c = v_x/c$, using \eqref{c5e39} and \eqref{c5e40}, we get
\begin{eqnarray}
H_x &=& 0 \label{c5e57} \\
H_y &=& -\frac{1}{c}v_xE_z \label{c5e58} \\
H_z &=& \frac{1}{c}v_xE_y. \label{c5e59}
\end{eqnarray}
These three equations can be combined as
\begin{equation}\label{c5e60}
\vec{H} = \frac{1}{c}\vec{v} \times \vec{E} = \vec{\beta} \times \vec{E}.
\end{equation}

\item We now consider the motion of a charge $q$ in the electric field produced
by another one $Q$. Let their masses by $m$ and $M$ respectively. Assume that
$m \ll M$ so that the charge $Q$ is almost stationary. The problem now reduces to
studying the motion of $q$ in a potential $\phi = Q/r$.

The energy of the charged particle is
\begin{equation}\label{c5e61}
\mathcal{E} = \sqrt{p^2c^2 + m^2c^4} + \frac{\alpha}{r},
\end{equation}
where
\begin{equation}\label{c5e62}
\alpha = qQ.
\end{equation}
The motion in a central field is confined to a plane. Align the coordinate axes
such that $Q$ is at the origin and the motion happens in $xy$ plane. Furthermore,
since the torque on the particle is zero, its angular momentum is a constant of
motion. The particle's velocity in polar coordinates is
\begin{equation}\label{c5e63}
\vec{v} = \dot{r}\uv{r} + r\dot{\theta}\uv{\theta}
\end{equation}
so that $v^2 = \dot{r}^2 + r^2\dot{\theta}^2$. Since $\vec{L} = \vec{r} \times
\vec{p} = m\gamma\vec{r} \times \vec{p}$, (using \eqref{c2e8}) we have $L = 
\gamma mr^2\dot{\theta}$. We can express $v^2$ in terms of $L$ as
\[
v^2 = \dot{r}^2 + \frac{L^2}{m^2\gamma^2 r^2}
\]
so that
\begin{equation}\label{c5e64}
p^2 = m^2\gamma^2\dot{r}^2 + \frac{L^2}{r^2} = p_r^2 + \frac{L^2}{r^2}.
\end{equation}
Therefore, \eqref{c5e61} becomes
\begin{equation}\label{c5e65}
\mathcal{E} = c\sqrt{p_r^2 + \frac{L^2}{r^2} + m^2c^2} + \frac{\alpha}{r}.
\end{equation}

\item If $\alpha > 0$ then as $r$ increases, the rhs of \eqref{c5e64} also
increases even if $p_r \rightarrow 0$. Since $\mathcal{E}$ is a constant of
motion, a drop in $r$ can be compensated by a drop in $p_r$ only to a limited
extent. This prevents the two charges from coming arbitrarily close to each 
other.

To analyse the condition $\alpha < 0$, write \eqref{c5e65} as
\[
\mathcal{E} = \frac{Lc}{r}\sqrt{\frac{r^2(p_r^2 + m^2c^2)}{L^2} + 1} - \frac{|\alpha|}{r}.
\]
so that we can approximate
\[
\mathcal{E} \approx \frac{Lc}{r} + \frac{cr}{2L}(p_r^2 + m^2c^2) - \frac{|\alpha|}{r}.
\]
for small $r$. If $Lc > |\alpha|$ then the rhs blows up as $r \rightarrow 0$. 
Therefore, to enforce constancy of $\mathcal{E}$, $r$ cannot be permitted to
decrease indefinitely. If $Lc < |\alpha|$, if $p_r = m\gamma\dot{r}$ can become
indefinitely large, $r$ may be allowed to become arbitrarily small while still
keeping $\mathcal{E}$ constant.

In the non-relativistic case, we would have had
\[
\mathcal{E} = \frac{1}{2}mv_r^2 + \frac{L^2}{2mr^2} - \frac{|\alpha|}{r}.
\]
If $L \ne 0$ then the first two terms, which are always positive, rise much faster
than the third term falls. Therefore, energy conservation does not allow the two
charges to come arbitrarily close to each other. On the other hand, if $L = 0$, 
then $v_r$ can rise enough to compensate the drop in the third term and still
keep  $\mathcal{E}$ constant. Thus, the two charges can come arbitrarily close only
if they approach to each other head-on.

\item The Hamilton-Jacobi equation \eqref{c3e15} for this problem is
\[
(\grad S)^2 - \frac{1}{c^2}\left(\pdt{S}{t} + \frac{\alpha}{r}\right)^2 + m^2c^2 = 0.
\]
Since $Q$ is stationary, $q$ experiences only the electric field and therefore 
$\vec{A} = 0$. The gradient in plane-polar coordinates is
\begin{equation}\label{c5e66}
\grad S = \pdt{S}{r}\uv{r} + \frac{1}{r}\pdt{S}{\phi}
\end{equation}
so that the Hamilton-Jacobi equation becomes
\begin{equation}\label{c5e67}
\left(\pdt{S}{r}\right)^2 + \frac{1}{r^2}\left(\pdt{S}{\phi}\right)^2 - \frac{1}{c^2}
\left(\pdt{S}{t} + \frac{\alpha}{r}\right)^2 + m^2c^2 = 0.
\end{equation}
or
\[
\left(\pdt{S}{r}\right)^2 + \frac{1}{r^2}\left(\pdt{S}{\phi}\right)^2 - \frac{1}{c^2}
\left(\pdt{S}{t}\right)^2 + 2\frac{\alpha}{rc^2}\pdt{S}{t} + \frac{\alpha^2}{c^2r^2}
+ m^2c^2 = 0.
\]
This is a non-linear, first-order pde. We try a solution of the form
\begin{equation}\label{c5e68}
S(r, \phi, t) = -\mathcal{E}t + L\phi + f(r)
\end{equation}
to get
\[
{f^\op(r)}^2 + \frac{L^2}{r^2} - \frac{\mathcal{E}^2}{c^2} - 2\frac{\alpha\mathcal{E}}{rc^2}
+ \frac{\alpha^2}{c^2r^2} + m^2c^2 = 0.
\]
or
\[
f^\op = \pm\sqrt{\frac{1}{c^2}\left(\mathcal{E} - \frac{\alpha}{r}\right)^2 - \frac{L^2}{r^2} 
-m^2c^2}
\]
The solution, thus, is
\begin{equation}\label{c5e69}
S(r, \phi, t) = -\mathcal{E}t + L\phi \pm 
\frac{1}{c}\int\sqrt{\left(\mathcal{E}-\frac{\alpha}{r}\right)^2-\frac{L^2c^2}{r^2} -m^2c^4}dr
\end{equation}
The trajectories are given by (find out why)
\begin{equation}\label{c5e70}
\pdt{S}{L} = \text{constant.}
\end{equation}
Differentiating \eqref{c5e69},
\begin{equation}\label{c5e71}
\pdt{S}{L} = \phi \mp Lc\int\frac{dr}{r\sqrt{A^2r^2 - 2Br + C^2}},
\end{equation}
where
\begin{eqnarray}
A^2 &=& \mathcal{E}^2 - m^2c^4 \label{c5e72} \\
B   &=& \alpha\mathcal{E} \label{c5e73} \\
C^2 &=& \alpha^2 - L^2c^2 \label{c5e74}
\end{eqnarray}
We now use the result
\begin{equation}\label{c5e75}
\int\frac{dx}{x\sqrt{a^2x^2 - 2bx + c^2}} = 
-\frac{1}{c}\tanh^{-1}\left(\frac{c^2 - bx}{c\sqrt{a^2x^2 - 2bx + c^2}}\right) +
\text{const}.
\end{equation}
in equation \eqref{c5e71} to get
\begin{equation}\label{c5e76}
\phi_0 = \phi \pm \frac{Lc}{C}\tanh^{-1}\left(\frac{C^2 - Br}{C\sqrt{A^2r^2 - 2Br + C^2}}\right),
\end{equation}
where $\phi_0$ is a constant of integration.

We consider the following cases:
\begin{enumerate}
\item $\alpha^2 > L^2c^2$, that is $C$ is real. Then \eqref{c5e71} can be written as
\[
\tanh\left(\frac{C}{Lc}(\phi_0 - \phi)\right) = \frac{C^2 - Br}{C\sqrt{A^2r^2 - 2Br + C^2}}.
\]
Let
\begin{equation}\label{c5e77}
X = \frac{C}{Lc}(\phi_0 - \phi) = \sqrt{\frac{\alpha^2}{L^2c^2} - 1}(\phi_0 - \phi)
\end{equation}
so that
\begin{eqnarray*}
\tanh^2 X &=& \frac{(C^2 - Br)^2}{C^2(A^2r^2 - 2Br + C^2)} \\
C^2(A^2r^2 + C^2 - 2Br)\tanh^2X &=& C^4 - 2BC^2r + B^2r^2 \\
C^2A^2r^2\tanh^2X &=& (C^4 - 2BC^2r)\sech^2X + B^2r^2 \\
C^2A^2r^2\sinh^2X &=& C^2(C^2 - 2B^2r) + B^2r^2\cosh^2X \\
C^2A^2r^2(\cosh^2X - 1) &=& C^2(C^2 - 2B^2r) + B^2r^2\cosh^2X \\
(C^2A^2 - B^2)r^2\cosh^2X &=& C^2(A^2r^2 - 2B^2r + C^2)
\end{eqnarray*}
Now,
\[
A^2C^2-B^2 = (L^2c^2 -\alpha^2)m^2c^4 -\mathcal{E}^2L^2c^2
\]
Since we assumes $\alpha^2 > L^2c^2$, the rhs of the above equation is negative.
Therefore, before taking the square-root, we flip the signs to get
\begin{eqnarray*}
(B^2 - C^2A^2)r^2\cosh^2X &=& C^2(2B^2r - A^2r^2 - C^2) \\
\sqrt{B^2 - C^2A^2}\cosh X &=& \frac{C^2}{r}\sqrt{2\frac{B^2}{C^2}r - \frac{A^2}{C^2}r^2 - 1}
\end{eqnarray*}
Thus,
\[
\pm c\sqrt{(L\mathcal{E})^2 + m^2c^2(\alpha^2 - L^2c^2)}\cosh X = 
\frac{C^2}{r}\sqrt{2\frac{B^2}{C^2}r - \frac{A^2}{C^2}r^2 - 1}
\]
Since $\cosh$ is an even function,
\begin{eqnarray}
\pm c\sqrt{(L\mathcal{E})^2 + m^2c^2(\alpha^2 - L^2c^2)}
\cosh\left((\phi - \phi_0)\sqrt{\frac{\alpha^2}{L^2c^2} - 1}\right) &=& \nonumber\\
\frac{C^2}{r}\sqrt{2\frac{B^2}{C^2}r - \frac{A^2}{C^2}r^2 - 1} \label{c5e78}
\end{eqnarray}
We can choose $\phi_0$ such that this equation reduces to
\begin{equation}\label{c5e79}
\pm c\sqrt{(L\mathcal{E})^2 + m^2c^2(\alpha^2 - L^2c^2)}
\cosh\left((\phi - \phi_0)\sqrt{\frac{\alpha^2}{L^2c^2} - 1}\right) = \frac{C}{r}.
\end{equation}
This can always be done because \eqref{c5e78} is of the form
\begin{equation}\label{c5e80}
A\cosh(B(x_0-x)) = Cf(x).
\end{equation}
We can write it as
\begin{equation}\label{c5e81}
x_0 = x + \frac{1}{B}\cosh^{-1}\left(\frac{Cf(x)}{A}\right).
\end{equation}
Choose $x_0$ such that if $f(x^\op) = 1$ then
\begin{equation}\label{c5e82}
x_0 = x^\op + \frac{1}{B}\cosh^{-1}\left(\frac{C}{A}\right).
\end{equation}
\end{enumerate}

\end{enumerate}