\documentclass{article}
\usepackage{amsmath, graphicx, xcolor, hyperref}
\usepackage{mathabx}
\include{common}
\begin{document}
\title{The Electric Potential}
\author{Amey Joshi}
\date{15-Jun-2024}
\maketitle
\begin{enumerate}
\item Given that $\vec{E} = 6xy\uv{x} + 3(x^2 - y^2)\uv{y}$. Denote the origin 
$(0,0,0)$ by $O$ and the point $(x_1, y_1, 0)$ by $A$. In the first case,
\begin{equation}\label{e1}
d\vec{s} = \uv{x}dx + \uv{y}dy
\end{equation}
so that the line integral is
\begin{eqnarray}
L_1 &=& \int_O^A\vec{E}\cdot d\vec{s} \nonumber \\
 &=& \int_0^{x_1}3x^2\uv{y}\cdot\uv{x}dx + 
     \int_0^{y_1}(6x_1y\uv{x} + 3(x_1^2 - y^2)\uv{y}dy)\cdot\uv{y}dy \nonumber \\
 &=& 0 + \int_0^{y_1}(x_1^2 - y^2)dy \nonumber \\
 &=& 3x_1^2y - y_1^3 \label{e2}
\end{eqnarray}
In the second case, the equation of the straight line is 
\begin{equation}\label{e3}
y = \frac{y_1}{x_1}x
\end{equation}
so that
\[
dy = \frac{y_1}{x_1}dx
\]
and
\begin{equation}\label{e4}
d\vec{s} = \uv{x}dx + \uv{y}dy = \uv{x}dx + \uv{y}\frac{y_1}{x_1}dx.
\end{equation}
Further, along the straight line,
\begin{equation}\label{e5}
\vec{E} = 6\frac{y_1}{x_1}x^2\uv{x} + 3\left(x^2 - \frac{y_1^2}{x_1^2}x^2\right)\uv{y}.
\end{equation}
so that the line integral is
\begin{eqnarray}
L_2 &=& \int_O^A\vec{E}\cdot d\vec{s} \nonumber \\
 &=& \int_O^A6\frac{y_1}{x_1}x^2dx + 
 3\left(x^2 - \frac{y_1^2}{x_1^2}x^2\right)\frac{y_1}{x_1}dx \nonumber \\
 &=& 2\frac{y_1}{x_1}x_1^3 + \frac{y_1}{x_1}\left(1 - \frac{y_1^2}{x_1^2}\right)x_1^3 \nonumber \\
 &=& 3x_1^2y_1 - y_1^3 \label{e6}
\end{eqnarray}
In the third case, $d\vec{s} = \uv{x}dx + \uv{y}dy$ and
\begin{eqnarray}
L_3 &=& -\int_0^{y_1}3y^2dy + \int_0^{x_1}6xy_1dx \nonumber \\
 &=& -y_1^3 + 3x_1^2y_1 \label{e7}
\end{eqnarray}
Equations \eqref{e2}, \eqref{e6} and \eqref{e7} show that the line integrals are
the same. The potential function is
\begin{equation}\label{e8}
\varphi(x, y, 0) = -\int_O^{(x, y, 0)}\vec{E}\cdot d\vec{s} = -(3x^2y - y^3).
\end{equation}
However,
\begin{equation}\label{e9}
\varphi(x, y, z) = -\int_O^{(x, y, z)}\vec{E}\cdot d\vec{s} = -(3x^2y - y^3).
\end{equation}
is also true (why?) so that
\[
-\grad\varphi = 6xy\uv{x} + 3(x^2-y^2)\uv{y} = \vec{E}.
\]

\item The potential of the charge configuration is
\begin{equation}\label{e10}
\varphi(0, 0, z) = 12/z - 6/(z - 3)
\end{equation}
so that the variation of potential is as shown in figure \ref{c2f2}. It was 
generated using
\begin{verbatim}
import numpy as np
import matplotlib.pyplot as plt

def varphi(z: float) -> float:
    return 12/z - 6/(z - 3)
    
Z1 = np.linspace(-6, 6)
Z2 = np.linspace(-0.1, 0.1)
Z3 = np.linspace(2.9, 3.1)

Z = np.concatenate((Z1, Z2, Z3))
Z.sort()
V = [varphi(z) for z in Z]

plt.plot(Z, V)
plt.xlabel(r'$z$')
plt.ylabel(r'$\varphi(0, 0, z)$')
plt.title('Potential due to two charges on the z-axis')
plt.show()
\end{verbatim}
\begin{figure}[!ht]
\center
\includegraphics[scale=0.6]{purcell_c2p2}
\caption{Problem 2}
\label{c2f2}
\end{figure}
A few points to consider:
\begin{itemize}
\item Examine its behaviour in the regions $z < 0, z \in (0, 3)$ and $z > 3$.
\item Why did we create three arrays $Z1, Z2, Z3$ in the code?
\item Why did we sort the array $Z$?
\end{itemize}

\item The potential at a point in the $y$ axis is
\begin{equation}\label{e11}
\varphi(y) = -\frac{2}{y} + \frac{1}{\sqrt{1 + (y - 1)^2}} + \frac{1}{\sqrt{1 + (y - 1)^2}} 
= -2\left(\frac{1}{y} - \frac{1}{\sqrt{1 + (y - 1)^2}}\right)
\end{equation}
Electric field $\vec{E} = -\grad\varphi$ will be zero when $d\varphi/dy = 0$. 
A few points to note about the potential:
\begin{itemize}
\item The function blows up at the origin.
\item For $y \rightarrow \pm \infty$, $\varphi(y) \rightarrow 0$.
\item For $y < 0$, $\varphi(y) > 0$.
\item $\varphi(0^+) = \infty, \varphi(1) = 0, \varphi(y) > 0$ for $y \in (0, 1) \cup (1, \infty)$.
\end{itemize}
Now,
\[
\td{\varphi}{z} = 2\left(\frac{1}{y^2} - \frac{(y - 1)}{(y^2 - 2y + 2)^{3/2}}\right)
\]
and $d\varphi/dz = 0$ implies $(y^2 - 2y + 2)^3 = y^4(y - 1)^2$. The roots of
\[
4 y^5 - 17 y^4 + 32 y^3 - 36 y^2 + 24 y - 8 = 0
\]
can be found using
\begin{verbatim}
np.roots([4, -17, 32, -36, 24, -8]).
\end{verbatim}
They are $y \approx 1.62072, 0.427249 \pm 0.974453 i, 0.887391 \pm 0.550058$. The only 
real root is $1.62072$.
The variation of the potential along the $y$ axis is shown in figure \ref{c2f3a} to 
\ref{c2f3e}.
\begin{figure}[!ht]
\center
\includegraphics[scale=0.75]{purcell_c2p3a}
\caption{In range $(-2, 2)$.}
\label{c2f3a}
\end{figure}
\begin{figure}[!ht]
\center
\includegraphics[scale=0.75]{purcell_c2p3b}
\caption{In range $(1.5, 1.7)$.}
\label{c2f3b}
\end{figure}
\begin{figure}[!ht]
\center
\includegraphics[scale=0.75]{purcell_c2p3c}
\caption{In range $(0.1, 2)$.}
\label{c2f3c}
\end{figure}
\begin{figure}[!ht]
\center
\includegraphics[scale=0.75]{purcell_c2p3d}
\caption{In range $(-5, -0.1)$.}
\label{c2f3d}
\end{figure}
\begin{figure}[!ht]
\center
\includegraphics[scale=0.75]{purcell_c2p3e}
\caption{In range $(1.5, 5)$.}
\label{c2f3e}
\end{figure}

The figures were generated using
\begin{verbatim}
import numpy as np
import matplotlib.pyplot as plt

def varphi(y: float) -> float:
    return -2 * (1/y - 1/np.sqrt(1 + (y - 1)**2))

def plot(ymin: float,
         ymax: float,
         fname: str,
         loc: str='best',
         show_x_axis: bool=True) -> None:
    Y = np.linspace(ymin, ymax)
    V = [varphi(y) for y in Y]
    label = f'In range [{ymin}, {ymax}]'
    plt.plot(Y, V, label=label)
    if show_x_axis:
        plt.hlines(y=0, xmin=ymin, xmax=ymax, color='red')
        
    plt.xlabel(r'$y$')
    plt.ylabel(r'$\varphi(y)$')
    plt.legend(loc=loc)
    plt.savefig(fname)
    plt.close()


def main():
    plot(-2, 2, 'course/purcell_c2p3a.png')
    plot(1.5, 1.7, 'course/purcell_c2p3b.png', show_x_axis=False)   
    plot(0.1, 2, 'course/purcell_c2p3c.png', loc='lower right')
    plot(-5, -0.1, 'course/purcell_c2p3d.png')
    plot(1, 5, 'course/purcell_c2p3e.png')


if __name__ == '__main__':
    main()

\end{verbatim}

\item Given the potential
\begin{equation}\label{e11}
\varphi(x, y, z) = \begin{cases}
x^2 + y^2 + z^2 \text{ for } x^2 + y^2 + z^2 < a^2 \\
-a^2 + \frac{2a^3}{\sqrt{x^2 + y^2 + z^2}} \text{ for } a^2 < x^2 + y^2 + z^2
\end{cases}
\end{equation}
the electric field $\vec{E} = -\grad\varphi$ is
\begin{equation}\label{e12}
\vec{E} = \begin{cases} -2(x\uv{x} + y\uv{y} + z\uv{z}) \text{ for } x^2 + y^2 + z^2 < a^2 \\
2a^3\frac{x\uv{x} + y\uv{y} + z\uv{z}}{(x^2 + y^2 + z^2)^{3/2}} \text{ for } a^2 < x^2 + y^2 + z^2
\end{cases}
\end{equation}
Therefore 
\begin{equation}\label{e13}
\dive\vec{E} = \begin{cases} -6 \text{ for } x^2 + y^2 + z^2 < a^2 \\
0 \text{ for } a^2 < x^2 + y^2 + z^2
\end{cases}
\end{equation}
so that, by Gauss law, the charge density is,
\begin{equation}\label{e14}
\rho = \begin{cases} -\frac{3}{2\pi} \text{ for } x^2 + y^2 + z^2 < a^2 \\
0 \text{ for } a^2 < x^2 + y^2 + z^2
\end{cases}
\end{equation}

\item Let $a$ be the radius of the sphere. If $Q$ is the total charge on it then
the potential at its surface is
\[
\varphi = -\frac{Q}{a}.
\]
If $\sigma$ is the surface charge density then $Q = 4\pi a^2\sigma$ so that
\[
\varphi = -4\pi a\sigma
\]
that is,
\[
\sigma = -\frac{\varphi}{4\pi a}.
\]
Given that $\varphi = 1000/300$ stat volt and electronic charge is $4.8 \times
10^{-10}$ esu, 
\[
\sigma = \frac{10}{3}\frac{1}{4\pi a}\frac{10^{10}}{4.8} \approx 
\frac{5.5}{a} \times 10^{-3} \times 10^{10} \approx \frac{5.5}{a} \times 10^7.
\]

\item The electric field on the surface of the earth is
\[
\vec{E} = \frac{1}{4\pi\epsilon_0}\frac{Q}{R^2}\uv{r}.
\]
Given that $R = 6.378 \times 10^6$ m,
\[
E \approx 9 \times 10^9 \times \frac{1}{4.078 \times 10^{13}} 
\approx 2.21 \times 10^{-4} \text{V/m}.
\]
The potential at the surface is
\[
\varphi = \frac{1}{4\pi\epsilon_0}\frac{Q}{R} \approx 1411 \text{V}.
\]

\item The integral,
\[
\int_C^D\vec{E}\cdot d\vec{s} = \varphi(D) - \varphi(C).
\]
It is easy to get the terms on the rhs.
\begin{eqnarray}
\varphi(C) &=& -\frac{2}{2\sqrt{5}} + \frac{3}{5} \label{e16} \\
\varphi(D) &=& -\frac{2}{5} + \frac{3}{2\sqrt{5}} \label{e17}
\end{eqnarray}
so that
\[
\int_C^D\vec{E}\cdot d\vec{s} = \frac{\sqrt{5} - 2}{2}.
\]

\item For the infinitely long cylinder of radius $a$ whose cross section is shown
in figure 2.17 of the book, the electric field is normal to the curved surface of
the cylinder. In order to get the field at a point which is at a distance $r$ from
the cylinder's axis, align the coordinates so that $z$ axis coincides with the 
cylinder's axis. Consider a pillbox coaxial with the cylinder and of radius $r$.
If $r < a$, the pillbox encloses a charge $\pi r^2 h \rho$, where $h$ is the
pillbox's height. The flux through the pillbox is $2\pi rh E$. Therefore, by
Gauss' law,
\[
2\pi rh E = 4\pi (\pi r^2h \rho)
\]
so that
\begin{equation}\label{e18}
\vec{E} = 2\pi\rho \vec{r}, \text{ if } r < a.
\end{equation}
If $r \ge a$, a similar analysis yields
\[
2\pi rh E = 4\pi (\pi a^2 h \rho)
\]
so that
\begin{equation}\label{e19}
\vec{E} = 2\pi\rho \frac{a^2}{r}\uv{r}, \text{ if } r \ge a.
\end{equation}
We are asked to find the potential assuming $\varphi(0) = 0$. Thus, if $r < a$,
\begin{equation}\label{e20}
\varphi(r) = \int_0^r\vec{E}\cdot d\vec{s} = 
\int_0^r 2\pi\rho \vec{r}^\op\cdot d\vec{r}^\op = \pi\rho r^2 \text{ if } r < a.
\end{equation}
If $r \ge a$,
\begin{eqnarray}
\varphi(r) &=& \int_0^r\vec{E}\cdot d\vec{s} \nonumber \\
 &=& \int_0^a\vec{E}\cdot d\vec{s} + \int_a^r\vec{E}\cdot d\vec{s} \nonumber \\
 &=& \pi\rho a^2 + 2\pi\rho a^2 \int_a^r \frac{dr^\op}{r^\op} \nonumber \\
 &=& \pi\rho a^2 + 2\pi\rho a^2\ln\left(\frac{r}{a}\right) \nonumber \\
 &=& \pi\rho a^2\left(1 + \ln\left(\frac{r^2}{a^2}\right)\right) \label{e21}
\end{eqnarray}
Note that $\varphi$ is continuous at $r = a$. So is the electric field.

\item The potential at the rim is $4\sigma a$ and that on the $y$ axis is 
\[
\varphi(0, y, 0) = 2\pi\sigma(\sqrt{y^2 + a^2} \pm y)
\]
so that the point on $y$ axis where the said equipotential cuts the $y$ axis
is given by the equation
\[
\pi(\sqrt{y^2 + a^2} \pm y) = 2 a.
\]
As expected, this equation is independent of $\sigma$. It is a purely geometrical
fact. I cannot sketch the equipotential surface without knowing its functional 
form. Finding $\varphi$ at an arbitrary point from the dissc is not a trivial 
problem.

\item The potential at a point on the $z$ axis is
\[
d\varphi(2d) = \frac{dq}{2d - z} = \lambda\frac{dz}{2d - z}
\]
so that
\begin{equation}\label{e22}
\varphi(2d) = \int_{-d}^d d\varphi(z) = -\int_{-d}^d\frac{dz}{z - 2d} = \lambda\ln 3
\end{equation}
For a point on the $x$ axis,
\[
d\varphi(x) = \frac{dq}{\sqrt{x^2 + z^2}}
\]
so that
\begin{eqnarray}
\varphi(x) &=& \lambda\int_{-d}^d\frac{dz}{\sqrt{x^2 + z^2}} \nonumber \\
 &=& \lambda\int_{-\alpha}^\alpha \sec\theta d\theta\;\text{ where }\alpha = \tan^{-1}(d/x) \nonumber \\
 &=& \lambda\ln|\sec\theta + \tan\theta|\Big|_{-\alpha}^\alpha \nonumber \\
 &=& \lambda\ln\left|\frac{\sqrt{x^2 + d^2} + d}{\sqrt{x^2 + d^2} - d}\right| \label{e23}
\end{eqnarray}
$\varphi(z = 2d) = \varphi(x)$ implies $\sqrt{x^2 + d^2} + d = 3(\sqrt{x^2 + d^2} - d)
\Rightarrow x = d\sqrt{3}$.

\item The distance between the point $P = (3d/2, 0, d)$ and a point $(0, 0, z)$ on
the rod is
\begin{equation}\label{e24}
r = \sqrt{\frac{9d^2}{4} + 0 + (d - z)^2}
\end{equation}
so that the potential at it due to a small charge element $dq$ at $z$ is
\[
d\varphi(P) = \frac{dq}{r} = 2\lambda\frac{dz}{\sqrt{9d^2 + 4(d - z)^2}}
\]
and 
\[
\varphi(P) = 2\lambda\int_{-d}^d\frac{dz}{\sqrt{9d^2 + 4(d - z)^2}}
\]
Let $u = 2(d - z)$ so that $du = -2dz$ and the limits of integral are from $u=4d$
to $z = 0$ and
\[
\varphi(P) = -\lambda\int_{4d}^0\frac{du}{\sqrt{9d^2 + u^2}}.
\]
If $u = 3d\tan\theta$ then $du = 3d\sec^2\theta d\theta$ and the limit of the 
integral are from $\alpha = \tan^{-1}(4/3)$ to $\theta = 0$.
\[
\varphi(P) = -\lambda\int_{\alpha}^0\sec\theta d\theta = 
-\lambda\ln|\sec\theta + \tan\theta|\Big|_{-\alpha}^0 =
-(0 - \lambda\ln 3) = \lambda\ln 3.
\]

We will repeat this analysis for an arbitrary point $Q = (X, 0, Z)$. Its distance 
from a point $(0, 0, z)$ on the rod is
\begin{equation}\label{e25}
r = \sqrt{X^2 + (Z - z)^2}
\end{equation}
so that the potential at it us
\[
\varphi(Q) = \lambda\int_{-d}^d\frac{dz}{\sqrt{X^2 + (Z - z)^2}}
\]
Let $u = Z - z$ so that $du = -dz$ and the limits of the integral go from
$Z + d$ to $Z - d$ and
\[
\varphi(Q) = -\lambda\int_{Z+d}^{Z-d}\frac{du}{\sqrt{X^2 + u^2}} = 
\lambda\int_{Z-d}^{Z+d}\frac{du}{\sqrt{X^2 + u^2}}.
\]
If $u = X\tan\theta$, $du = X\sec^2\theta d\theta$ and the limits of the
integral become 
\[
\alpha = \tan^{-1}\left(\frac{Z - d}{X}\right) \;\text{and}\;
\beta = \tan^{-1}\left(\frac{Z + d}{X}\right).
\]
We then have,
\[
\varphi(Q) = \lambda\int_\alpha^\beta \sec\theta d\theta = 
\lambda\ln|\sec\theta + \tan\theta|\Big|_\alpha^\beta.
\]
Now,
\[
\tan\alpha = \frac{Z-d}{X} \Rightarrow \sec\alpha=\frac{\sqrt{X^2 + (Z-d)^2}}{X}
\]
so that
\[
\varphi(Q) = \lambda\ln\left|\frac{\sqrt{X^2 + (Z+d)^2} + Z+d}{X}\right| - 
\lambda\ln\left|\frac{\sqrt{X^2 + (Z-d)^2} + Z-d}{X}\right|
\]
or
\begin{equation}\label{e26}
\varphi(Q) = \lambda\ln\left|\frac{\sqrt{X^2 + (Z+d)^2} + Z+d}{\sqrt{X^2 + (Z-d)^2} + Z-d}\right|
\end{equation}
$\varphi(Q)$ will be equal to $\varphi(P)$ when
\[
\frac{\sqrt{X^2 + (Z+d)^2} + Z+d}{\sqrt{X^2 + (Z-d)^2} + Z-d} = \sqrt{3}
\]
In general, if $\varphi(P) = k$ then the equation of the equipotential line is
\begin{equation}\label{e27}
\sqrt{X^2 + (Z+d)^2} + Z+d = k\sqrt{X^2 + (Z-d)^2} + kZ - kd.
\end{equation}
If
\begin{equation}\label{e28}
\frac{X^2}{a^2 - d^2} + \frac{Z^2}{a^2} = 1
\end{equation}
then
\begin{equation}\label{e29}
X^2 = a^2 - Z^2 - d^2 + \frac{Z^2d^2}{a^2}
\end{equation}
and
\[
X^2 + (Z \pm d)^2 = a^2 + \frac{Z^2d^2}{a^2} \pm 2Zd = \left(\frac{Zd}{a} \pm a\right)^2.
\]
Substituting this in \eqref{e27}, we get
\begin{equation}\label{e30}
\frac{Zd}{a} + a + Z + d = k\left(\frac{Zd}{a} - a\right) + kZ - kd,
\end{equation}
that is
\[
(k + 1)(a + d) = (k - 1)Z\frac{a + d}{a} \Rightarrow a(k + 1) = (k - 1)Z.
\]
Thus, if
\begin{equation}\label{e31}
Z = \frac{k + 1}{k - 1}a,
\end{equation}
then the point $(X, Z)$ lies on the ellipse defined by \eqref{e28}.

\item Refer to figure 2.12 of the book. We will first find the potential due to
the shaded strip in it. Let $q$ be the charge on it, $h$ be its height and $x$
be its distance from $P$. The potential due to a charge element $dq$ at height
$y$ at $P$ is
\[
\varphi(P) = \frac{dq}{r} = \lambda\frac{dy}{\sqrt{x^2 + y^2}}
\]
and 
\[
\varphi(P) = \lambda\int_0^h\frac{dy}{\sqrt{x^2 + y^2}} = 
\lambda\int_0^\theta\sec\psi d\psi,
\]
where $y = x\tan\psi$ and $\theta = \tan^{-1}(h/x)$. Thus,
\begin{equation}\label{e32}
\varphi(P) = \frac{q}{h}\ln|\sec\theta + \tan\theta|.
\end{equation}
To extend this solution to the potential due to the triangular region, let
the strip by of height $h$ and thickness $dx$ so that the charge on it is
$dq = \sigma hdx$ and we have
\[
d\varphi(P) = \sigma dx\ln|\sec\theta + \tan\theta|
\]
and
\begin{equation}\label{e33}
\varphi(P) = \int_0^b\sigma dx\ln|\sec\theta + \tan\theta| = 
\sigma b\ln|\sec\theta + \tan\theta|.
\end{equation}

\item It is easy to check that $\curl\vec{E} = 0$.

\item $\nabla^2 f \ne 0, \nabla^2 g = 0$. Further $\grad g = 2(x\uv{x} - y\uv{y})$.
The Hessian determinant of $g$ is a constant, $-4$. Since it is negative, all extrema
are saddle points.

The function $f$, on the other hand, is an elliptic paraboloid. Since $\grad f = 
2(x\uv{x} - y\uv{y})$, the origin $(0, 0)$ is a global extremum. The Hessian 
determinant at $(0, 0)$ is $4$ and $g_{xx} = g_{yy} = 2 > 0$. Therefore, the 
extremum is indeed a minimum.

\item 
\begin{enumerate}
\item If $\vec{F} = (x + y)\uv{x} + (-x + y)\uv{y} - 2z\uv{z}$, $\dive\vec{F} = 0$
and $\curl\vec{F} = -2\uv{x}$.

\item If $\vec{G} = 2y\uv{x} + (2x + 3z)\uv{y} + 3y\uv{z}$, $\dive\vec{G} = 0$ and
$\curl\vec{G} = 0$. Therefore, we can find a function $\varphi$ such that $\vec{G}
= \grad\varphi$. The field $\vec{G}$ vanishes at the origin. If we assume that the
potential also vanishes there,
\[
\varphi(x, y, z) = \int_{(0, 0, 0)}^{(x, y, z)} \vec{G}(x^\op, y^\op, z^\op)\cdot d\vec{s},
\]
along any curve joining the limits of the integral. Choose a curve composed of the
straight lines $(0, 0, 0)$ to $(x, 0, 0)$, $(x, 0, 0)$ to $(x, y, 0)$ and $(x, y, 0)$
to $(x, y, z)$. The field takes the forms $2x^\op\uv{y}$, $2y^\op\uv{x} + 2x\uv{y}
+ 3y^\op\uv{z}$ and $2y\uv{x} + (2x + 3z^\op)\uv{y} + 3y\uv{z}$ along the three
lines. Then,
\begin{eqnarray*}
\varphi(x, y, z) &=& \int_{(0, 0, 0)}^{(x, 0, 0)}\vec{G}\cdot\uv{x}dx +
\int_{(x, 0, 0)}^{(x, y, 0)}\vec{G}\cdot\uv{y}dy + 
\int_{(x, y, 0)}^{(x, y, z)}\vec{G}\cdot\uv{z}dz \\
 &=& 0 + 2x\int_{(x, 0, 0)}^{(x, y, 0)} dy^\op + 3y\int_{(x, y, 0)}^{(x, y, z)} dz^\op \\
 &=& 2xy + 3yz.
\end{eqnarray*}
We confirm that $\grad\varphi = 2y\uv{x} + (2x + 3z)\uv{y} + 3y\uv{z} = \vec{G}$.

\item If $\vec{H} = (x^2 - z^2)\uv{x} + 2\uv{y} + 2xz\uv{z}$ then $\dive\vec{H}
 = 4x$ and $\curl\vec{H} = -4z\uv{y}$.
\end{enumerate}

\item Part (a) is a straightforward manipulation in Cartesian coordinates. The
second method is superior because the proof is independent of the coordinates.
In figure 2.16 of the book, let the volume $V$ be composed of the top portion
$V_1$ and the bottom portion $V_2$. Let the surface $S$ be common to both.
Then,
\begin{eqnarray*}
\int_V\dive\curl\vec{A}\;dv &=& \int_{V_1}\dive\curl\vec{A}\;dv + 
  \int_{V_2}\dive\curl\vec{A}\;dv \\
  &=& \int_{S_1}\curl\vec{A}\cdot d\vec{a} + \int_{S_2}\curl\vec{A}\cdot d\vec{a},
\end{eqnarray*}
where $S_1$ and $S_2$ are closed surfaces that include the outer surface and the
one enclosed by the curve $C$ in the figure. Since they are both closed surfaces,
\[
\int_V\dive\curl\vec{A}\;dv = \int_{C_1}\vec{A}\cdot d\vec{s} + 
\int_{C_2}\vec{A}\cdot d\vec{s} = 0 + 0
\]
Since this is true for any volume $V$, we have $\dive\curl\vec{A} = 0$.

\item We have to prove the equivalence of
\begin{equation}\label{e34}
U = \frac{1}{8\pi}\int E^2 dv
\end{equation}
and
\begin{equation}\label{e35}
U = \frac{1}{2}\int\rho\varphi dv
\end{equation}
for a charge distribution of \emph{finite extent}. If $\varphi$ is the potential
due to the distribution $\rho$,
\[
\int_V \dive(\varphi\grad\varphi)dv = \int_S \varphi\grad\varphi\cdot d\vec{a}.
\]
Choose $V$ to be very large so that on the bounding surface $S$, $\varphi$ goes
as $r^{-1}$, $\grad\varphi$ as $r^{-2}$ and the area itself as $r^2$. Thus, if $S$
is very far from the charge distribution, which we are assured to be of finite
extend, then the surface integral can be made vanishingly small. Thus,
\[
\int_V \dive(\varphi\grad\varphi)dv = 0.
\]
Since $\dive(\varphi\grad\varphi) = |\grad\varphi|^2 + \varphi\nabla^2\varphi =
E^2 - 4\pi\varphi\rho$,
\[
\int_V E^2 dv = 4\pi\int\rho\varphi dv
\]
from which the equivalence of \eqref{e34} and \eqref{e35} follows.

The idea of choosing a very large volume to integrate over a function that is
non-zero over a finite region in space so that the transformed surface integral
is zero is very common in physics.

\item We will find the potential at an arbitrary point on the axis of the cylinder.
Align the axes such that the $z$ axis coincides with the cylinder's principal axis 
and the origin is at a distance $b/2$ from either extremity.

The potential due to a ring of charge at distance $r$ from the field point 
$(0, 0, z_0)$ is
\[
d\varphi = \frac{dq}{r} = \frac{\sigma \times 2\pi adz}{\sqrt{a^2 + (z - z_0)^2}}
\]
and
\[
\varphi(z_0) = 2\pi a\sigma\int_{-b/2}^{b/2}\frac{dz}{\sqrt{a^2 + (z - z_0)^2}}.
\]
Let $(z - z_0) = a\tan\theta$ so that $dz = a\sec^2\theta d\theta$ and the limits
of the integral are from
\[
\alpha = \tan^{-1}\left(\frac{-b-2z_0}{2a}\right)  \text{ to } 
\beta = \tan^{-1}\left(\frac{b - 2z_0}{2a}\right).
\]
Therefore,
\[
\varphi(z_0) = 2\pi a\sigma\ln\left|\frac{\sec\beta + \tan\beta}{\sec\alpha + \tan\alpha}\right|.
\]
Substituting for $\alpha$ and $\beta$ we get
\[
\varphi(z_0) = 2\pi a\sigma\ln\left|\frac{\sqrt{4a^2 + (b - 2z_0)^2} + b - 2z_0}{\sqrt{4a^2 + (b + 2z_0)^2} + b + 2z_0}\right|
\]
Note that when $\tan\alpha < 0$ then so is $\sec\alpha$ so that the denominator 
is really the sum of two negative terms whose modulus is the sum of corresponding
positive terms. In general, we can write
\begin{equation}\label{e36}
\varphi(z) = 2\pi a\sigma\ln\left|\frac{\sqrt{4a^2 + (b - 2z)^2} + b - 2z}{\sqrt{4a^2 + (b + 2z)^2} + b + 2z}\right|
\end{equation}
Clearly,
\begin{eqnarray*}
\varphi(b/2) &=& 2\pi a\sigma\ln\left|\frac{a}{\sqrt{a^2+b^2} + b}\right| \\
\varphi(0) &=& 0 \\
\varphi(-b/2) &=& 2\pi a\sigma\ln\left|\frac{\sqrt{a^2+b^2} + b}{a}\right|
\end{eqnarray*}
Therefore,
\begin{eqnarray*}
\varphi(b/2) - \varphi(0) &=& 2\pi a\sigma\ln\left|\frac{a}{\sqrt{a^2+b^2} + b}\right| \\
\varphi(0) - \varphi(-b/2) &=& 2\pi a\sigma\ln\left|\frac{\sqrt{a^2+b^2} + b}{a}\right| \\
 &=& 2\pi a\sigma\ln\left|\frac{a}{\sqrt{a^2+b^2} + b}\right| \\
 &=& \varphi(b/2) - \varphi(0)
\end{eqnarray*}
\end{enumerate}

\section{Potential of a uniformly charged disc}
The textbook mentions that the potential at arbitrary points due to a uniformly
charged disc can be expressed in terms of elliptic functions. We will derive the
expresions here following the paper (\href{https://arxiv.org/pdf/2004.04540}{pre-print})\cite{bs}.
\subsection{Arbitrary point on the disc}
\subsection{Arbitrary point not on the disc}

\begin{thebibliography}{1}
\bibitem{bs} On the electrostatic potential and electric field of a uniformly charged disk.
published in the European Journal of Physics 41.4 (2020): 045201
\end{thebibliography}
\end{document}